finish chapter 14 exercises

software-foundations/logical-foundations/ch12-imperative-programs/EvaluationFunction.v
@@ -5,3 +5,140 @@
   "imperative programs".
 *)
 
+Require Import Utf8.
+Require Import State.
+Require Import String.
+Require Import TotalMap.
+
+Notation "'LETOPT' x <== e1 'IN' e2"
+   := (match e1 with
+         | Some x => e2
+         | None => None
+       end)
+   (right associativity, at level 60).
+
+Open Scope imp_scope.
+
+Fixpoint ceval_step (st : state) (c : com) (i : nat)
+                    : option state :=
+  match i with
+  | O    => None
+  | S i' =>
+    match c with
+    | SKIP     => Some st
+    | l ::= a1 => Some (l !-> aeval st a1 ; st)
+    | c1 ;; c2 =>
+        LETOPT st' <== ceval_step st c1 i' IN
+          ceval_step st' c2 i'
+    | TEST b THEN c1 ELSE c2 FI =>
+        if (beval st b)
+        then ceval_step st c1 i'
+        else ceval_step st c2 i'
+    | WHILE b1 DO c1 END =>
+        if (beval st b1)
+        then LETOPT st' <== ceval_step st c1 i' IN
+               ceval_step st' c i'
+        else Some st
+    end
+  end.
+Close Scope imp_scope.
+
+Definition test_ceval (st:state) (c:com) :=
+  match ceval_step st c 500 with
+  | None    => None
+  | Some st => Some (st X, st Y, st Z)
+  end.
+
+Definition pup_to_n : com :=
+  Y ::= 0 ;; 
+  WHILE (¬ X = 0) DO
+    Y ::= Y + X ;;
+    X ::= X - 1
+  END.
+
+Example pup_to_n_1 :
+  test_ceval (X !-> 5) pup_to_n
+  = Some (0, 15, 0).
+Proof. reflexivity. Qed.
+
+Definition peven : com :=
+  Z ::= X ;;
+  WHILE 2 ≤ Z DO
+    Z ::= Z - 2
+  END
+.
+
+Example peven_test_1 : test_ceval (X !-> 0) peven = Some (0, 0, 0).
+Proof. reflexivity. Qed.
+
+Example peven_test_2 : test_ceval (X !-> 1) peven = Some (1, 0, 1).
+Proof. reflexivity. Qed.
+
+Example peven_test_3 : test_ceval (X !-> 4) peven = Some (4, 0, 0).
+Proof. reflexivity. Qed.
+
+Example peven_test_4 : test_ceval (X !-> 11) peven = Some (11, 0, 1).
+Proof. reflexivity. Qed.
+
+Theorem ceval_step__ceval: ∀c st st',
+  (∃i, ceval_step st c i = Some st') → st =[ c ]=> st'.
+Proof.
+  intros c st st' [i H].
+  generalize dependent st.
+  generalize dependent st'.
+  generalize dependent c.
+  induction i; intros. simpl. inversion H.
+  destruct c; simpl in H. 
+  - inversion H as [Hst]. apply E_Skip.
+  - inversion H as [Hst]. apply E_Ass. reflexivity.
+  - destruct (ceval_step st  c1 i) as [st1 |] eqn: E1; try
+    destruct (ceval_step st1 c2 i) as [st2 |] eqn: E2; inversion H as [Hst].
+    subst st2. apply E_Seq with st1; apply IHi; assumption.
+  - destruct (beval st b) eqn: EB.
+    1: apply E_IfTrue. 3: apply E_IfFalse.
+    all: try apply IHi; assumption.
+  - destruct (beval st b) eqn: EB.
+    + destruct (ceval_step st  c i) as [st1 |] eqn: E1; try
+      destruct (ceval_step st1 (WHILE b DO c END) i) as [st2 |] eqn: E2;
+      inversion H as [Hst]. subst st2.
+      apply E_WhileTrue with st1. exact EB.
+      all: (apply IHi; assumption).
+    + inversion H. subst st.
+      apply E_WhileFalse. exact EB.
+Qed.
+
+Require Import Omega.
+
+(* Proof is given by the textbook *)
+Axiom ceval_step_more: ∀i1 i2 st st' c,
+  i1 ≤ i2 → ceval_step st c i1 = Some st' → ceval_step st c i2 = Some st'.
+
+Theorem ceval__ceval_step: ∀ c st st',
+  st =[ c ]=> st' → ∃ i, ceval_step st c i = Some st'.
+Proof.
+  intros c st st' H. induction H;
+  try
+  ( destruct IHceval1 as [n1 Hst1]
+  ; destruct IHceval2 as [n2 Hst2]
+  ; apply ceval_step_more with (i2 := n1 + n2) in Hst1
+  ; apply ceval_step_more with (i2 := n1 + n2) in Hst2
+  );
+  try omega;
+  try destruct IHceval as [n Hst].
+  - exists 1. reflexivity.
+  - exists 1. simpl. rewrite H. reflexivity.
+  - exists (S (n1 + n2)). simpl. 
+    rewrite Hst1. exact Hst2.
+  - exists (S n). simpl. rewrite H. exact Hst.
+  - exists (S n). simpl. rewrite H. exact Hst.
+  - exists 1. simpl. rewrite H. reflexivity.
+  - exists (S (n1 + n2)). simpl. rewrite H.
+    rewrite Hst1. exact Hst2.
+Qed.
+
+Theorem ceval_and_ceval_step_coincide: ∀ c st st',
+  st =[ c ]=> st' ↔ ∃ i, ceval_step st c i = Some st'.
+Proof.
+  intros. split.
+  apply ceval__ceval_step. apply ceval_step__ceval.
+Qed.
